src/Assembly/GF25519.v
@@ -1,5 +1,4 @@
 Require Import Crypto.Assembly.Pipeline.
-
 Require Import Crypto.Spec.ModularArithmetic.
 Require Import Crypto.ModularArithmetic.ModularBaseSystem.
 Require Import Crypto.Specific.GF25519.
@@ -9,8 +8,7 @@ Module GF25519.
   Definition bits: nat := 64.
   Definition width: Width bits := W64.
 
-  Instance ZE : Evaluable Z := @ZEvaluable bits.
-  Existing Instance ZE.
+  Existing Instance ZEvaluable.
 
   Fixpoint makeBoundList {n} k (b: @BoundedWord n) :=
     match k with
@@ -35,24 +33,141 @@ Module GF25519.
     exact t.
   Defined.
 
-  Definition flatten {T}: (@interp_type Z FE -> T) -> NAry 10 Z T.
-    intro F; refine (fun (a b c d e f g h i j: Z) =>
-      F (a, b, c, d, e, f, g, h, i, j)).
-  Defined.
+  Section Expressions.
+    Definition flatten {T}: (@interp_type Z FE -> T) -> NAry 10 Z T.
+      intro F; refine (fun (a b c d e f g h i j: Z) =>
+        F (a, b, c, d, e, f, g, h, i, j)).
+    Defined.
 
-  Definition unflatten {T}:
+    Definition unflatten {T}:
       (forall a b c d e f g h i j, T (a, b, c, d, e, f, g, h, i, j))
     -> (forall x: @interp_type Z FE, T x).
-  Proof.
-    intro F; refine (fun (x: @interp_type Z FE) =>
-      let '(a, b, c, d, e, f, g, h, i, j) := x in
-      F a b c d e f g h i j).
-  Defined.
+    Proof.
+      intro F; refine (fun (x: @interp_type Z FE) =>
+        let '(a, b, c, d, e, f, g, h, i, j) := x in
+        F a b c d e f g h i j).
+    Defined.
 
-  Ltac intro_vars_for R := revert R;
-    match goal with
-    | [ |- forall x, @?T x ] => apply (@unflatten T); intros
-    end.
+    Ltac intro_vars_for R := revert R;
+      match goal with
+      | [ |- forall x, @?T x ] => apply (@unflatten T); intros
+      end.
+
+    Definition ge25519_add_expr :=
+      Eval cbv beta delta [fe25519 carry_add mul carry_sub opp Let_In] in carry_add.
+
+    Definition ge25519_sub_expr :=
+      Eval cbv beta delta [fe25519 carry_add mul carry_sub opp Let_In] in carry_sub.
+
+    Definition ge25519_mul_expr :=
+      Eval cbv beta delta [fe25519 carry_add mul carry_sub opp Let_In] in mul.
+
+    Definition ge25519_opp_expr :=
+      Eval cbv beta delta [fe25519 carry_add mul carry_sub opp Let_In] in opp.
+
+    Definition ge25519_add' (P Q: @interp_type Z FE):
+      { r: @HL.Expr Z FE | HL.Interp r = ge25519_add_expr P Q }.
+    Proof.
+      intro_vars_for P.
+      intro_vars_for Q.
+
+      eexists.
+
+      cbv beta delta [ge25519_add_expr].
+
+      etransitivity; [reflexivity|].
+
+      let R := HL.rhs_of_goal in
+      let X := HL.Reify R in
+      transitivity (HL.Interp (X bits)); [reflexivity|].
+
+      cbv iota beta delta [ HL.Interp
+          interp_type interp_binop HL.interp
+          Z.land ZEvaluable eadd esub emul eshiftr eand].
+
+      reflexivity.
+    Defined.
+
+    Definition ge25519_sub' (P Q: @interp_type Z FE):
+      { r: @HL.Expr Z FE | HL.Interp r = ge25519_sub_expr P Q }.
+    Proof.
+      intro_vars_for P.
+      intro_vars_for Q.
+
+      eexists.
+
+      cbv beta delta [ge25519_sub_expr].
+
+      etransitivity; [reflexivity|].
+
+      let R := HL.rhs_of_goal in
+      let X := HL.Reify R in
+      transitivity (HL.Interp (X bits)); [reflexivity|].
+
+      cbv iota beta delta [ HL.Interp
+          interp_type interp_binop HL.interp
+          Z.land ZEvaluable eadd esub emul eshiftr eand].
+
+      reflexivity.
+    Defined.
+
+    Definition ge25519_mul' (P Q: @interp_type Z FE):
+      { r: @HL.Expr Z FE | HL.Interp r = ge25519_mul_expr P Q }.
+    Proof.
+      intro_vars_for P.
+      intro_vars_for Q.
+
+      eexists.
+
+      cbv beta delta [ge25519_mul_expr].
+
+      etransitivity; [reflexivity|].
+
+      let R := HL.rhs_of_goal in
+      let X := HL.Reify R in
+      transitivity (HL.Interp (X bits)); [reflexivity|].
+
+      cbv iota beta delta [ HL.Interp
+          interp_type interp_binop HL.interp
+          Z.land ZEvaluable eadd esub emul eshiftr eand].
+
+      reflexivity.
+    Defined.
+
+    Definition ge25519_opp' (P: @interp_type Z FE):
+      { r: @HL.Expr Z FE | HL.Interp r = ge25519_opp_expr P }.
+    Proof.
+      intro_vars_for P.
+
+      eexists.
+
+      cbv beta delta [ge25519_opp_expr zero_].
+
+      etransitivity; [reflexivity|].
+
+      let R := HL.rhs_of_goal in
+      let X := HL.Reify R in
+      transitivity (HL.Interp (X bits)); [reflexivity|].
+
+      cbv iota beta delta [ HL.Interp
+          interp_type interp_binop HL.interp
+          Z.land ZEvaluable eadd esub emul eshiftr eand].
+
+      reflexivity.
+    Defined.
+
+    Definition ge25519_add (P Q: @interp_type Z FE) :=
+        proj1_sig (ge25519_add' P Q).
+
+    Definition ge25519_sub (P Q: @interp_type Z FE) :=
+        proj1_sig (ge25519_sub' P Q).
+
+    Definition ge25519_mul (P Q: @interp_type Z FE) :=
+        proj1_sig (ge25519_mul' P Q).
+
+    Definition ge25519_opp (P: @interp_type Z FE) :=
+        proj1_sig (ge25519_opp' P).
+  End Expressions.
 
   Module AddExpr <: Expression.
     Definition bits: nat := bits.
@@ -61,32 +176,7 @@ Module GF25519.
     Definition ResultType := FE.
     Definition inputBounds := feBound ++ feBound.
 
-    Definition ge25519_add_expr :=
-        Eval cbv beta delta [fe25519 carry_add mul carry_sub Let_In] in carry_add.
-
-    Definition ge25519_add' (P Q: @interp_type Z FE) :
-        { r: @HL.expr Z (@interp_type Z) FE | HL.interp (t := FE) r = ge25519_add_expr P Q }.
-    Proof.
-      intro_vars_for P.
-      intro_vars_for Q.
-
-      eexists.
-      cbv beta delta [ge25519_add_expr].
-
-      let R := HL.rhs_of_goal in
-      let X := HL.reify (@interp_type Z) R in
-      transitivity (HL.interp (t := ResultType) X); [reflexivity|].
-
-      cbv iota beta delta [
-            interp_type interp_binop HL.interp
-            Z.land ZEvaluable eadd esub emul eshiftr eand].
-      reflexivity.
-    Defined.
-
-    Definition ge25519_add (P Q: @interp_type Z ResultType) :=
-        proj1_sig (ge25519_add' P Q).
-
-    Definition hlProg: NAry 20 Z (@HL.expr Z (@interp_type Z) ResultType) :=
+    Definition prog: NAry 20 Z (@HL.Expr Z ResultType) :=
         Eval cbv in (flatten (fun p => (flatten (fun q => ge25519_add p q)))).
   End AddExpr.
 
@@ -98,31 +188,10 @@ Module GF25519.
     Definition inputBounds := feBound ++ feBound.
 
     Definition ge25519_sub_expr :=
-        Eval cbv beta delta [fe25519 carry_add mul carry_sub Let_In] in carry_sub.
+      Eval cbv beta delta [fe25519 carry_add mul carry_sub opp Let_In] in
+        carry_sub.
 
-    Definition ge25519_sub' (P Q: @interp_type Z FE) :
-        { r: @HL.expr Z (@interp_type Z) FE | HL.interp (t := FE) r = ge25519_sub_expr P Q }.
-    Proof.
-      intro_vars_for P.
-      intro_vars_for Q.
-
-      eexists.
-      cbv beta delta [ge25519_sub_expr].
-
-      let R := HL.rhs_of_goal in
-      let X := HL.reify (@interp_type Z) R in
-      transitivity (HL.interp (t := ResultType) X); [reflexivity|].
-
-      cbv iota beta delta [
-            interp_type interp_binop HL.interp
-            Z.land ZEvaluable eadd esub emul eshiftr eand].
-      reflexivity.
-    Defined.
-
-    Definition ge25519_sub (P Q: @interp_type Z ResultType) :=
-        proj1_sig (ge25519_sub' P Q).
-
-    Definition hlProg: NAry 20 Z (@HL.expr Z (@interp_type Z) ResultType) :=
+    Definition prog: NAry 20 Z (@HL.Expr Z ResultType) :=
         Eval cbv in (flatten (fun p => (flatten (fun q => ge25519_sub p q)))).
   End SubExpr.
 
@@ -133,32 +202,7 @@ Module GF25519.
     Definition ResultType := FE.
     Definition inputBounds := feBound ++ feBound.
 
-    Definition ge25519_mul_expr :=
-        Eval cbv beta delta [fe25519 carry_add mul carry_sub Let_In] in mul.
-
-    Definition ge25519_mul' (P Q: @interp_type Z FE) :
-        { r: @HL.expr Z (@interp_type Z) FE | HL.interp (t := FE) r = ge25519_mul_expr P Q }.
-    Proof.
-      intro_vars_for P.
-      intro_vars_for Q.
-
-      eexists.
-      cbv beta delta [ge25519_mul_expr].
-
-      let R := HL.rhs_of_goal in
-      let X := HL.reify (@interp_type Z) R in
-      transitivity (HL.interp (t := ResultType) X); [reflexivity|].
-
-      cbv iota beta delta [
-            interp_type interp_binop HL.interp
-            Z.land ZEvaluable eadd esub emul eshiftr eand].
-      reflexivity.
-    Defined.
-
-    Definition ge25519_mul (P Q: @interp_type Z ResultType) :=
-        proj1_sig (ge25519_mul' P Q).
-
-    Definition hlProg: NAry 20 Z (@HL.expr Z (@interp_type Z) ResultType) :=
+    Definition prog: NAry 20 Z (@HL.Expr Z ResultType) :=
         Eval cbv in (flatten (fun p => (flatten (fun q => ge25519_mul p q)))).
   End MulExpr.
 
@@ -169,34 +213,8 @@ Module GF25519.
     Definition ResultType := FE.
     Definition inputBounds := feBound.
 
-    Definition ge25519_opp_expr :=
-        Eval cbv beta delta [fe25519 carry_add mul carry_sub carry_opp Let_In] in carry_opp.
-
-    Definition ge25519_opp' (P: @interp_type Z FE) :
-        { r: @HL.expr Z (@interp_type Z) FE
-        | HL.interp (E := @ZEvaluable bits) (t := FE) r = ge25519_opp_expr P }.
-    Proof.
-      intro_vars_for P.
-
-      eexists.
-      cbv beta delta [ge25519_opp_expr zero_].
-
-      let R := HL.rhs_of_goal in
-      let X := HL.reify (@interp_type Z) R in
-      transitivity (HL.interp (E := @ZEvaluable bits) (t := ResultType) X);
-        [reflexivity|].
-
-      cbv iota beta delta [
-        interp_type interp_binop HL.interp
-        Z.land ZEvaluable eadd esub emul eshiftr eand].
-      reflexivity.
-    Defined.
-
-    Definition ge25519_opp (P: @interp_type Z ResultType) :=
-        proj1_sig (ge25519_opp' P).
-
-    Definition hlProg: NAry 10 Z (@HL.expr Z (@interp_type Z) ResultType) :=
-        Eval cbv in (flatten (fun p => ge25519_opp p)).
+    Definition prog: NAry 10 Z (@HL.Expr Z ResultType) :=
+        Eval cbv in (flatten ge25519_opp).
   End OppExpr.
 
   Module Add := Pipeline AddExpr.
@@ -204,11 +222,6 @@ Module GF25519.
   Module Mul := Pipeline MulExpr.
   Module Opp := Pipeline OppExpr.
 End GF25519.
-
-Set Printing All.
-Opaque eadd esub emul eshiftr eand toT fromT.
-Eval cbv iota beta delta in GF25519.Add.HL.progZ.
-Eval cbv iota beta delta in GF25519.Add.AST.progZ.
 
 Extraction "GF25519Add" GF25519.Add.
 Extraction "GF25519Sub" GF25519.Sub.
